theories/clang/lib/page_table.v
@@ -18,13 +18,13 @@ Structure page_table Σ `{!clangG Σ} :=  {
   (* -- operation specs -- *)
   insert_pt_spec i l m Φ:
     is_page_table m ∗ (is_page_table (<[ i := l ]> m) -∗ Φ Vvoid)
-    ⊢ WP (Ecall_typed Tvoid insert_pt [Evalue (Vint32 i); Evalue (Vptr l)]) {{ Φ }};
+    ⊢ WP (Ecall Tvoid insert_pt [Evalue (Vint32 i); Evalue (Vptr l)]) {{ Φ }};
   delete_pt_spec i m Φ:
     is_page_table m ∗ (is_page_table (delete i m) -∗ Φ Vvoid)
-    ⊢ WP (Ecall_typed Tvoid delete_pt [Evalue (Vint32 i)]) {{ Φ }};
+    ⊢ WP (Ecall Tvoid delete_pt [Evalue (Vint32 i)]) {{ Φ }};
   lookup_pt_spec i m Φ:
     is_page_table m ∗ (is_page_table m -∗ Φ (option_addr_to_val (m !! i)))
-    ⊢ WP (Ecall_typed (Tptr Tvoid) lookup_pt [Evalue (Vint32 i)]) {{ Φ }}
+    ⊢ WP (Ecall (Tptr Tvoid) lookup_pt [Evalue (Vint32 i)]) {{ Φ }}
 }.
 
 Arguments insert_pt {_ _} _.
