theories/clang/lib/vmm.v
@@ -7,10 +7,10 @@ Section vmm.
 
   Definition mem_init (n: nat) (x: addr) (y: addr) : expr :=
     x <- 0 ;;
-    while [ !x@Tint32 :<: n ] ( !x@Tint32 :<: n ) <{
+    while: ( !x@Tint32 :<: n ) (
       y <- Ealloc (Tprod Tint8 Tvoid) (Vpair vfalse Vvoid) ;;
-      Ecall_typed Tvoid (insert_pt pt) [!x@Tint32 ; Evalue (Vptr y)]
-    }>.
+      Ecall Tvoid (insert_pt pt) [!x@Tint32 ; Evalue (Vptr y)]
+    ).
 
   Fixpoint allocated (m: gmap int32 addr) (n: nat) : iProp Σ :=
     match m !! Int.repr n with
