theories/clang/notations.v
@@ -28,16 +28,15 @@ Notation "e1 != e2" := (Ebinop oneq e1%E e2%E)
   (at level 50, left associativity) : expr_scope.
 Notation "e1 :<: e2" := (Ebinop oless e1%E e2%E)
   (at level 50, left associativity) : expr_scope.
-Notation "f # t <$ e1 , e2 , .. , en $>" := (Ecall_typed t f (cons e1%E (cons e2%E .. (cons en%E nil) .. )))
-  (at level 50) : expr_scope.
-
 Notation "e1 <- e2" := (Eassign e1%E e2%E) (at level 80) : expr_scope.
-Notation "'if:' ( e ) then: { s1 } 'else:' { s2 }" := (Eif e%E s1%E s2%E)
+Notation "'if:' ( e ) then: ( s1 ) 'else:' ( s2 ) " := (Eif e%E s1%E s2%E)
   (at level 200, e, s1, s2 at level 200) : expr_scope.
-Notation "'while' [ c ] ( e ) <{ s }>" := (Ewhile c%E e%E s%E)
-  (at level 200, c, e, s at level 200) : expr_scope.
+Notation "'while:' ( e ) ( s ) " := (Ewhile e%E e%E s%E)
+  (at level 200, e, s at level 200) : expr_scope.
 Notation "s1 ;; s2" := (Eseq s1%E s2%E)
   (at level 100, s2 at level 200, format "s1  ;;  s2") : expr_scope.
 Notation "'return:' e" := (Erete e%E) (at level 80): expr_scope.
-Notation "'let:' x ::: t := e1 'in' e2" := (Elet_typed t x e1%E e2%E)
+Notation "'let:' x ::: t := e1 'in' e2" := (Elet t x e1%E e2%E)
   (at level 102, x, t at level 1, e1, e2 at level 200) : expr_scope.
+Notation "'let:' x ::: t 'in' e2" := (Edecl t x e2%E)
+  (at level 102, x, t at level 1, e2 at level 200) : expr_scope.
