theories/tests/higher_order.v
@@ -3,21 +3,18 @@ Require Import iris_c.clang.logic.
 Section example.
   Context `{clangG Σ}.
 
-  Definition f (g: ident) : expr :=
-    Ecall_typed Tvoid g [].
-
   Definition abs_spec g E (P Q: iProp Σ) :=
     (∃ gbody, text_interp g (Function Tvoid [] gbody) ∗
               (∀ Φ, P -∗ (Q -∗ Φ Vvoid) -∗ WP gbody @ E {{ Φ }}))%I.
 
-  Lemma f_spec ks E g Φ P Q:
+  Lemma higher_order_spec ks E g Φ P Q:
     abs_spec g E P Q ∗ P ∗
     own_stack ks ∗ (own_stack ([]::ks) -∗ Q -∗ Φ Vvoid)
-    ⊢ WP f g @ E {{ Φ }}.
+    ⊢ WP Ecall Tvoid g [] @ E {{ Φ }}.
   Proof.
     iIntros "(Hg & HP & Hs & HΦ)".
     iDestruct "Hg" as (e) "[Ht He]".
-    unfold f. iApply (wp_call [] []); last iFrame; first done.
+    iApply (wp_call [] []); last iFrame; first done.
     iNext. iIntros "Hs'".
     iApply ("He" with "HP").
     by iApply "HΦ".
